FlatStack/FlatStackLanguage.thy
@@ -13,16 +13,16 @@ type_synonym flat_stack_state = "int list \<times> flat_stack_instruction list \
 
 inductive eval_flat_stack :: "flat_stack_program \<Rightarrow> flat_stack_state \<Rightarrow> flat_stack_state \<Rightarrow> bool" where
   evf_jump [simp]: "\<Pi> s = Some (\<pi>, s') \<Longrightarrow> eval_flat_stack \<Pi> (\<sigma>, [], s, \<omega>) (\<sigma>, \<pi>, s', \<omega>)"
-| evf_add [simp]: "eval_flat_stack \<Pi> (i1 # i2 # \<sigma>, FAdd # \<pi>, s, \<omega>) ((i2 + i1) # \<sigma>, \<pi>, s, \<omega>)"
+| evf_add [simp]: "eval_flat_stack \<Pi> (i1 # i2 # \<sigma>, FAdd # \<pi>, s, \<omega>) ((i1 + i2) # \<sigma>, \<pi>, s, \<omega>)"
 | evf_sub [simp]: "eval_flat_stack \<Pi> (i1 # i2 # \<sigma>, FSub # \<pi>, s, \<omega>) ((i2 - i1) # \<sigma>, \<pi>, s, \<omega>)"
 | evf_neg [simp]: "eval_flat_stack \<Pi> (i1 # \<sigma>, FNeg # \<pi>, s, \<omega>) ((-i1) # \<sigma>, \<pi>, s, \<omega>)"
 | evf_eq [simp]: "eval_flat_stack \<Pi> (i1 # i2 # \<sigma>, FEq # \<pi>, s, \<omega>) (unboolify (i2 = i1) # \<sigma>, \<pi>, s, \<omega>)"
 | evf_gt [simp]: "eval_flat_stack \<Pi> (i1 # i2 # \<sigma>, FGt # \<pi>, s, \<omega>) (unboolify (i2 > i1) # \<sigma>, \<pi>, s, \<omega>)"
 | evf_lt [simp]: "eval_flat_stack \<Pi> (i1 # i2 # \<sigma>, FLt # \<pi>, s, \<omega>) (unboolify (i2 < i1) # \<sigma>, \<pi>, s, \<omega>)"
 | evf_and [simp]: "eval_flat_stack \<Pi> (i1 # i2 # \<sigma>, FAnd # \<pi>, s, \<omega>) 
-    (unboolify (boolify i2 \<and> boolify i1) # \<sigma>, \<pi>, s, \<omega>)"
+    (unboolify (boolify i1 \<and> boolify i2) # \<sigma>, \<pi>, s, \<omega>)"
 | evf_or [simp]: "eval_flat_stack \<Pi> (i1 # i2 # \<sigma>, FOr # \<pi>, s, \<omega>) 
-    (unboolify (boolify i2 \<or> boolify i1) # \<sigma>, \<pi>, s, \<omega>)"
+    (unboolify (boolify i1 \<or> boolify i2) # \<sigma>, \<pi>, s, \<omega>)"
 | evf_not [simp]: "eval_flat_stack \<Pi> (i1 # \<sigma>, FNot # \<pi>, s, \<omega>) 
     (unboolify (\<not> boolify i1) # \<sigma>, \<pi>, s, \<omega>)"
 | evf_print [simp]: "eval_flat_stack \<Pi> (i1 # \<sigma>, FPrint # \<pi>, s, \<omega>) (\<sigma>, \<pi>, s, i1 # \<omega>)"
